Reworking eval tactic a bit

SkLean/EvalTactic.lean
@@ -5,6 +5,7 @@ import Lean.Expr
 
 open Lean Meta Qq
 open PrettyPrinter
+open Elab Tactic
 
 declare_syntax_cat skmexprquot
 syntax "K"                                                             : skmexprquot
@@ -31,101 +32,108 @@ macro_rules
     << $e₂ >>)
   | `(<< ($e:skmexprquot) >>)            => `(<<$e>>)
 
--- Closes a goal of the form `beta_eq e₁ e₂` by recursively evaluating the expression
-partial def eval_to (from_e : Lean.Expr) (to_e : Option Lean.Expr) : OptionT MetaM $ List Lean.Expr := do
-  if (← (to_e.map $ isDefEq from_e).getD (pure false)) then
-    pure [(Lean.Expr.const `beta_eq.rfl []),]
-  else match (← whnf from_e) with
-    | SKM`[((K x) _y)] =>
-      pure $ ([
-        (Lean.Expr.const `beta_eq.trans []),
-        (Lean.Expr.const `beta_eq.eval []),
-        (Lean.Expr.const `is_eval_once.k []),
-      ]) ++ (← eval_to x to_e)
-    | SKM`[(((S x) y) z)] =>
-      pure $ ([
-        (Lean.Expr.const `beta_eq.trans []),
-        (Lean.Expr.const `beta_eq.eval []),
-        (Lean.Expr.const `is_eval_once.s []),
-      ]) ++ (← eval_to SKM`[((x z) (y z))] to_e)
-    | SKM`[(M K)] =>
-      let e' ← OptionT.mk (pure $ (← getConstInfo `t_k).value?)
-
-      pure $ ([
-        (Lean.Expr.const `beta_eq.trans []),
-        (Lean.Expr.const `beta_eq.eval []),
-        (Lean.Expr.const `is_eval_once.m_k []),
-      ]) ++ (← eval_to e' to_e)
-    | SKM`[(M M)] =>
-      let e' ← OptionT.mk (pure $ (← getConstInfo `t_m).value?)
-
-      pure $ ([
-        (Lean.Expr.const `beta_eq.trans []),
-        (Lean.Expr.const `beta_eq.eval []),
-        (Lean.Expr.const `is_eval_once.m_m []),
-      ]) ++ (← eval_to e' to_e)
-    | SKM`[(M S)] =>
-      let e' ← OptionT.mk (pure $ (← getConstInfo `t_s).value?)
-
-      pure $ ([
-        (Lean.Expr.const `beta_eq.trans []),
-        (Lean.Expr.const `beta_eq.eval []),
-        (Lean.Expr.const `is_eval_once.m_s []),
-      ]) ++ (← eval_to e' to_e)
-    | SKM`[(M (e₁ e₂))] =>
-      let t_out ← OptionT.mk (pure $ (← getConstInfo `t_out).value?)
-      let e' := SKM`[(t_out ((M e₁) e₂))]
-
-      pure $ [
-        (Lean.Expr.const `beta_eq.trans []),
-        (Lean.Expr.const `beta_eq.eval []),
-        (Lean.Expr.const `is_eval_once.m_call [])
-      ] ++ (← eval_to e' to_e)
-    | SKM`[(lhs rhs)] =>
-      pure $ [
-        (Lean.Expr.const `beta_eq.trans []),
-        (Lean.Expr.const `beta_eq.left [])]
-          ++ (← eval_to lhs none)
-          ++ [
-            (Lean.Expr.const `beta_eq.trans []),
-            (Lean.Expr.const `beta_eq.right [])]
-          ++ (← eval_to rhs none)
-    | SKM`[K] => pure [Lean.Expr.const `beta_eq.rfl []]
-    | SKM`[S] => pure [Lean.Expr.const `beta_eq.rfl []]
-    | SKM`[M] => pure [Lean.Expr.const `beta_eq.rfl []]
-    | _ => pure []
-
-def parse_beta_eq_call (e : Lean.Expr) : OptionT MetaM $ Lean.Expr × Lean.Expr := do
+def parse_beta_eq_call (e : Lean.Expr) : TacticM (Option (Lean.Expr × Lean.Expr)) := do
   let e ← whnf e
   match e with
     | .app (.app (.const `beta_eq []) from_e) to_e =>
-      pure $ ⟨from_e, to_e⟩
+      pure $ pure ⟨from_e, to_e⟩
     | _ =>
-      OptionT.mk (pure .none)
+      (pure .none)
+
+def get_goal_target_e  : TacticM (Option Lean.Expr) := do
+  let goal   ← getMainGoal
+  let goal_e := (← Term.getMVarDecl goal).type
+
+  let some ⟨_, to_e⟩ ← parse_beta_eq_call goal_e | return none
+
+  if to_e.hasMVar then
+    pure none
+  else
+    pure to_e
+
+def get_goal_from_e  : TacticM (Option Lean.Expr) := do
+  let goal   ← getMainGoal
+  let goal_e := (← Term.getMVarDecl goal).type
+
+  let some ⟨from_e, _⟩ ← parse_beta_eq_call goal_e | return none
+
+  pure from_e
+
+-- Closes a goal of the form `beta_eq e₁ e₂` by recursively evaluating the expression
+partial def eval_to (to_e : Option Lean.Expr) : TacticM (Option Unit):= do
+  let do_apply : List Lean.Expr → TacticM Unit := fun (exprs) => do
+    exprs.forM (fun (e) => do
+      let e' ← delab e
+      evalTactic (← `(tactic| apply $e'))
+    )
+
+  let some from_e := (← get_goal_from_e) | return ()
+
+  let to_e ← (do match ← get_goal_target_e with
+    | .some g => do
+      let _ ← do_apply [(Lean.Expr.const `beta_eq.trans [])]
+      pure $ .some g
+    | .none =>
+      pure to_e)
+
+  if (← liftMetaM (to_e.mapM $ isDefEq from_e)).getD false then
+    do_apply [(Lean.Expr.const `beta_eq.rfl []),]
+  else match (← whnf from_e) with
+    | SKM`[((K x) _y)] =>
+      let _ ← do_apply [
+        Lean.Expr.const `beta_eq.eval [],
+        Lean.Expr.const `is_eval_once.k [],
+      ]
+      eval_to to_e
+    | SKM`[(((S x) y) z)] =>
+      let _ ← do_apply [
+        (Lean.Expr.const `beta_eq.eval []),
+        (Lean.Expr.const `is_eval_once.s []),
+      ]
+      eval_to to_e
+    | SKM`[(M K)] =>
+      let _ ← do_apply [
+        (Lean.Expr.const `beta_eq.eval []),
+        (Lean.Expr.const `is_eval_once.m_k []),
+      ]
+      eval_to to_e
+    | SKM`[(M M)] =>
+      let _ ← do_apply [
+        (Lean.Expr.const `beta_eq.eval []),
+        (Lean.Expr.const `is_eval_once.m_m []),
+      ]
+      eval_to to_e
+    | SKM`[(M S)] =>
+      let _ ← do_apply [
+        (Lean.Expr.const `beta_eq.eval []),
+        (Lean.Expr.const `is_eval_once.m_s []),
+      ]
+      eval_to to_e
+    | SKM`[(M (e₁ e₂))] =>
+      let _ ← do_apply [
+        (Lean.Expr.const `beta_eq.eval []),
+        (Lean.Expr.const `is_eval_once.m_call []),
+      ]
+      eval_to to_e
+    | SKM`[K] => do_apply [Lean.Expr.const `beta_eq.rfl []]
+    | SKM`[S] => do_apply [Lean.Expr.const `beta_eq.rfl []]
+    | SKM`[M] => do_apply [Lean.Expr.const `beta_eq.rfl []]
+    | SKM`[(lhs rhs)] =>
+      let _ ← do_apply [
+        (Lean.Expr.const `beta_eq.left [])]
+      let _ ← eval_to lhs
+      let _ ← do_apply [
+             Lean.Expr.const `beta_eq.right []]
+      eval_to none
+    | _ => pure $ pure ()
 
 syntax "eval_to" ( term ) : tactic
 
-open Elab Tactic
 elab_rules : tactic
-  | `(tactic| eval_to $e) => do
-    let e' ← (((do
-    let goal      ← getMainGoal
-    let goal_e := (← Term.getMVarDecl goal).type
-    let ⟨from_e, _⟩ ← OptionT.mk (pure $ ← liftMetaM $ parse_beta_eq_call goal_e)
+  | `(tactic| eval_to $e) => (do
     let to_e ← elabTerm e none
 
-    let exprs ← liftMetaM $ eval_to from_e to_e
-
-    match exprs with
-      | Option.some exprs =>
-        for e in exprs do
-          logInfo s!"{e}"
-          let e_stx ← delab e
-          evalTactic (← `(tactic| apply $e_stx))
-      | .none =>
-        return ()) : OptionT TacticM Unit)
-          |> OptionT.run)
-    pure $ e'.getD ()
+    eval_to to_e).bind (fun o => pure $ o.getD ())
 
 example : beta_eq SKM[((K x) y)] x := by
   eval_to x
@@ -136,6 +144,11 @@ example : beta_eq SKM[((K (K K)) K)] SKM[(K K)] := by
 example : beta_eq SKM[(((S K) K) K)] SKM[K] := by
   eval_to SKM[K]
 
-example : beta_eq SKM[(M ((K K) K))] SKM[(t_out ((M (K K)) K))] := by
-  eval_to SKM[(t_out ((M (K K)) K))]
+example : beta_eq SKM[(M (((S K) K) K))] SKM[(t_out ((M ((S K) K)) K))] := by
+  eval_to SKM[(t_out ((M ((S K) K)) K))]
+
+example : beta_eq SKM[(M (((S K) K) K))] SKM[(M K)] := by
+  eval_to SKM[(M K)]
+  trace_state
+
 
